File.v
@@ -6,16 +6,16 @@ Require Import FileIds.
 Require Import Util.
 
 Open Local Scope bool.
-Open Local Scope Z.
+Open Local Scope N.
 
 Structure File := mkFile {
   fileId: FileId;
-  fileSize: Z;
+  fileSize: N;
   deleted: bool;
-  lastAccess: Exc Z;
-  lastModification: Exc Z;
-  lastCreated: Exc Z;
-  lastDeleted: Exc Z
+  lastAccess: Exc N;
+  lastModification: Exc N;
+  lastCreated: Exc N;
+  lastDeleted: Exc N
 }.
 
 Definition isDeleted (file: File) := 
@@ -25,10 +25,10 @@ Definition eqb (lhs rhs: File) :=
   (FileIds.eqb lhs.(fileId) rhs.(fileId))
   && (lhs.(fileSize) =? rhs.(fileSize))
   && (Bool.eqb lhs.(deleted) rhs.(deleted))
-  && (optZ_eqb lhs.(lastAccess) rhs.(lastAccess))
-  && (optZ_eqb lhs.(lastModification) rhs.(lastModification))
-  && (optZ_eqb lhs.(lastCreated) rhs.(lastCreated))
-  && (optZ_eqb lhs.(lastDeleted) rhs.(lastDeleted)).
+  && (optN_eqb lhs.(lastAccess) rhs.(lastAccess))
+  && (optN_eqb lhs.(lastModification) rhs.(lastModification))
+  && (optN_eqb lhs.(lastCreated) rhs.(lastCreated))
+  && (optN_eqb lhs.(lastDeleted) rhs.(lastDeleted)).
 
 Lemma eqb_reflection (lhs rhs: File):
   eqb lhs rhs = true -> lhs = rhs.
@@ -44,12 +44,12 @@ Proof.
   destruct lhs. destruct rhs. 
   simpl in H, H0, H1, H2, H3, H4, H5.
   apply eqb_reflection in H. rewrite H. clear H.
-  apply Z.eqb_eq in H5. rewrite H5. clear H5.
+  apply N.eqb_eq in H5. rewrite H5. clear H5.
   apply -> Bool.eqb_true_iff in H4. rewrite H4. clear H4.
-  apply optZ_eqb_reflection in H0. rewrite H0. clear H0.
-  apply optZ_eqb_reflection in H1. rewrite H1. clear H1.
-  apply optZ_eqb_reflection in H2. rewrite H2. clear H2.
-  apply optZ_eqb_reflection in H3. rewrite H3. clear H3.
+  apply optN_eqb_reflection in H0. rewrite H0. clear H0.
+  apply optN_eqb_reflection in H1. rewrite H1. clear H1.
+  apply optN_eqb_reflection in H2. rewrite H2. clear H2.
+  apply optN_eqb_reflection in H3. rewrite H3. clear H3.
   reflexivity.
 Qed.
 
@@ -64,7 +64,7 @@ Proof.
     destruct rhs ; [| discriminate H | discriminate H].
       apply eqb_reflection in H. rewrite H. reflexivity.
     destruct rhs ; [discriminate H | | discriminate H].
-      apply Z.eqb_eq in H. rewrite H. reflexivity.
+      apply N.eqb_eq in H. rewrite H. reflexivity.
     destruct rhs ; [discriminate H | discriminate H |].
       discriminate H.
 Qed.
