FileIds.v
@@ -3,15 +3,15 @@ Require Import Coq.ZArith.ZArith.
 Require Import ByteData.
 
 Inductive FileId: Type :=
-  | Ext2Id: Z -> FileId
-  | TarId: FileId -> Z -> FileId
+  | Ext2Id: N -> FileId
+  | TarId: FileId -> N -> FileId
   | MockId: ByteData -> FileId
 .
 
 Fixpoint eqb (lhs rhs: FileId) :=
   match (lhs, rhs) with
-  | ((Ext2Id l), (Ext2Id r)) => Z.eqb l r
-  | ((TarId lfs l), (TarId rfs r)) => (andb (eqb lfs rfs) (Z.eqb l r))
+  | ((Ext2Id l), (Ext2Id r)) => N.eqb l r
+  | ((TarId lfs l), (TarId rfs r)) => (andb (eqb lfs rfs) (N.eqb l r))
   | _ => false
   end.
 
@@ -23,13 +23,13 @@ Proof.
     (* Ext2Id *)
     destruct rhs0; 
       [| simpl; intros; inversion H | simpl; intros; inversion H].
-    unfold eqb. intros. apply Z.eqb_eq in H. rewrite H. reflexivity.
+    unfold eqb. intros. apply N.eqb_eq in H. rewrite H. reflexivity.
     (* TarId *)
     destruct rhs0; 
       [simpl; intros; inversion H | | simpl; intros; inversion H].
       intros. unfold eqb in H. 
       apply Bool.andb_true_iff in H. destruct H.
-      apply Z.eqb_eq in H0. rewrite H0.
+      apply N.eqb_eq in H0. rewrite H0.
       apply IHlhs in H. rewrite H.
       reflexivity.
     (* MockId *)
