Util.v
@@ -4,11 +4,12 @@ Require Import Coq.Strings.String.
 Require Import Coq.ZArith.ZArith.
 Require Export List.
 
+Require Import Byte.
 Require Import ByteData.
 Require Import Fetch.
 
-Open Local Scope bool.
-Open Local Scope Z.
+Local Open Scope bool.
+Local Open Scope N.
 
 (* Functional programming idioms *)
 Definition flatmap {A B: Type} (opt: Exc A) (fn: A -> Exc B) 
@@ -25,7 +26,7 @@ Definition opt_map {A B: Type} (opt: Exc A) (fn: A -> B)
     | None => None
   end.
 
-Definition opt_eqbZ (lhs rhs: Exc Z): bool :=
+Definition opt_eqbN (lhs rhs: Exc N): bool :=
   match (lhs, rhs) with
   | (Some l, Some r) => l =? r
   | (None, None) => true
@@ -35,15 +36,15 @@ Definition opt_eqbZ (lhs rhs: Exc Z): bool :=
 Infix "_flatmap_" := flatmap (at level 50).
 Infix "_map_" := opt_map (at level 50).
 
-Definition range (start: Z) (exclusiveEnd: Z) : list Z :=
+Definition range (start: N) (exclusiveEnd: N) : list N :=
   N.peano_rect
-  (fun _ => Z -> list Z) (* Signature of recursive calls *)
-  (fun (start: Z) => nil) (* Base case *)
-  (fun (counter: N) (rec: Z -> list Z) (start: Z) =>
+  (fun _ => N -> list N) (* Signature of recursive calls *)
+  (fun (start: N) => nil) (* Base case *)
+  (fun (counter: N) (rec: N -> list N) (start: N) =>
     if (exclusiveEnd <=? start)
     then nil
     else start :: (rec (start + 1)))
-  (Z.to_N (exclusiveEnd - start))
+  (exclusiveEnd - start)
   start.
 
 Infix "upto" := range (at level 50).
@@ -68,16 +69,16 @@ Fixpoint flatten {A} (lst: list (Exc A)): list A :=
 
 (* from a Disk, extract the list of elements
   [ disk start; disk (start + 1); ... ; disk (start + length - 1) ] *)
-Definition seq_list (disk: Disk) (start length: Z): @Fetch (list Z) :=
+Definition seq_list (disk: Disk) (start length: N): @Fetch (list Byte) :=
   match length with
-    | Z0 => Found nil
-    | Zpos l => 
+    | 0 => Found nil
+    | N.pos l => 
       (Pos.peano_rec
-        (fun _ => Z -> @Fetch (list Z))
-        (fun (start': Z) => (disk start') _fmap_ (fun nextEl => nextEl :: nil))
-        (fun _ (seq_list_aux_pred_l: Z -> @Fetch (list Z)) (start': Z) => 
+        (fun _ => N -> @Fetch (list Byte))
+        (fun (start': N) => (disk start') _fmap_ (fun nextEl => nextEl :: nil))
+        (fun _ (seq_list_aux_pred_l: N -> @Fetch (list Byte)) (start': N) => 
           (disk start') _fflatmap_ (fun nextEl =>
-            (seq_list_aux_pred_l (Z.succ start')) _fmap_ (fun tail =>
+            (seq_list_aux_pred_l (N.succ start')) _fmap_ (fun tail =>
               nextEl :: tail
             )
           )
@@ -85,27 +86,26 @@ Definition seq_list (disk: Disk) (start length: Z): @Fetch (list Z) :=
       )
       l
       start
-    | Zneg _ => MissingAt length (* Should never be reached *)
   end.
 
 (* little endian unsigned *)
-Fixpoint lendu (l : list Z) : Z := 
+Fixpoint lendu (l : list Byte) : N := 
 match l with 
   | nil => 0
-  | a :: l' => (a + (256 * lendu l'))
+  | a :: l' => (N_of_ascii a) + (256 * lendu l')
 end.   
 
-Definition seq_lendu (disk: Disk) (offset: Z) (length: Z): @Fetch Z :=
+Definition seq_lendu (disk: Disk) (offset: N) (length: N): @Fetch N :=
   (seq_list disk offset length) _fmap_ (fun tail => lendu tail).
 
-Fixpoint listZ_eqb (l r: list Z) := match (l, r) with
+Fixpoint listN_eqb (l r: list N) := match (l, r) with
   | (nil, nil) => true
-  | (l :: ltail, r :: rtail) => (andb (l =? r) (listZ_eqb ltail rtail))
+  | (l :: ltail, r :: rtail) => (andb (l =? r) (listN_eqb ltail rtail))
   | (_, _) => false
 end.
 
-Lemma listZ_eqb_reflection (l r: list Z) :
-  listZ_eqb l r = true <-> l = r.
+Lemma listN_eqb_reflection (l r: list N) :
+  listN_eqb l r = true <-> l = r.
 Proof.
   split. (* -> *)
     generalize r.
@@ -117,9 +117,9 @@ Proof.
     destruct r0.
       inversion H.
 
-      unfold listZ_eqb in H.
+      unfold listN_eqb in H.
       apply Bool.andb_true_iff in H. destruct H.
-      apply Z.eqb_eq in H. rewrite H.
+      apply N.eqb_eq in H. rewrite H.
       apply IHl in H0. rewrite H0.
       reflexivity.
   (* <- *)
@@ -132,25 +132,24 @@ Proof.
     destruct r0.
       inversion H.
       
-      unfold listZ_eqb. apply Bool.andb_true_iff.
+      unfold listN_eqb. apply Bool.andb_true_iff.
       inversion H.
       split.
-        apply Z.eqb_eq. reflexivity.
+        apply N.eqb_eq. reflexivity.
         rewrite <- H2 at 1. apply IHl in H2. auto.
 Qed.
 
-Definition optZ_eqb (lhs rhs: Exc Z) := match (lhs, rhs) with
+Definition optN_eqb (lhs rhs: Exc N) := match (lhs, rhs) with
   | (None, None) => true
   | (Some l, Some r) => l =? r
   | _ => false
 end.
 
-Lemma optZ_eqb_reflection (lhs rhs: Exc Z) :
-  optZ_eqb lhs rhs = true -> lhs = rhs.
+Lemma optN_eqb_reflection (lhs rhs: Exc N) :
+  optN_eqb lhs rhs = true -> lhs = rhs.
 Proof.
-  intros. unfold optZ_eqb in H.
+  intros. unfold optN_eqb in H.
   destruct lhs. 
-    destruct rhs; [|discriminate H]. apply Z.eqb_eq in H. rewrite H. reflexivity.
+    destruct rhs; [|discriminate H]. apply N.eqb_eq in H. rewrite H. reflexivity.
     destruct rhs; [discriminate H|]. auto.
 Qed.
- 
