Byte.v
@@ -1,0 +1,67 @@
+Require Import Coq.Strings.Ascii.
+Require Import Coq.ZArith.ZArith.
+
+Require Import Fetch.
+
+Definition Byte := ascii.
+
+Local Open Scope bool.
+
+Definition eqb (lhs rhs: Byte) : bool :=
+  match (lhs, rhs) with
+  | (Ascii l1 l2 l3 l4 l5 l6 l7 l8, Ascii r1 r2 r3 r4 r5 r6 r7 r8) =>
+      (Bool.eqb l1 r1) && (Bool.eqb l2 r2)
+      && (Bool.eqb l3 r3) && (Bool.eqb l4 r4)
+      && (Bool.eqb l5 r5) && (Bool.eqb l6 r6)
+      && (Bool.eqb l7 r7) && (Bool.eqb l8 r8)
+  end.
+
+Lemma eqb_reflection (lhs rhs: Byte) :
+  eqb lhs rhs = true <-> lhs = rhs.
+Proof.
+  split. (* -> *)
+    intros. unfold eqb in H.
+    destruct lhs. destruct rhs.
+    apply Bool.andb_true_iff in H. destruct H. 
+    apply Bool.andb_true_iff in H. destruct H. 
+    apply Bool.andb_true_iff in H. destruct H. 
+    apply Bool.andb_true_iff in H. destruct H. 
+    apply Bool.andb_true_iff in H. destruct H. 
+    apply Bool.andb_true_iff in H. destruct H. 
+    apply Bool.andb_true_iff in H. destruct H. 
+    apply Bool.eqb_prop in H; rewrite H; clear H.
+    apply Bool.eqb_prop in H0; rewrite H0; clear H0.
+    apply Bool.eqb_prop in H1; rewrite H1; clear H1.
+    apply Bool.eqb_prop in H2; rewrite H2; clear H2.
+    apply Bool.eqb_prop in H3; rewrite H3; clear H3.
+    apply Bool.eqb_prop in H4; rewrite H4; clear H4.
+    apply Bool.eqb_prop in H5; rewrite H5; clear H5.
+    apply Bool.eqb_prop in H6; rewrite H6; clear H6.
+    reflexivity.
+  (* <- *)
+    intros. unfold eqb.
+    destruct lhs. destruct rhs. inversion H. 
+    apply Bool.andb_true_iff. split; [| apply Bool.eqb_reflx].
+    apply Bool.andb_true_iff. split; [| apply Bool.eqb_reflx].
+    apply Bool.andb_true_iff. split; [| apply Bool.eqb_reflx].
+    apply Bool.andb_true_iff. split; [| apply Bool.eqb_reflx].
+    apply Bool.andb_true_iff. split; [| apply Bool.eqb_reflx].
+    apply Bool.andb_true_iff. split; [| apply Bool.eqb_reflx].
+    apply Bool.andb_true_iff. split; [| apply Bool.eqb_reflx].
+    apply Bool.eqb_reflx.
+Qed.
+
+
+Definition feqb (lhs rhs: @Fetch Byte) := Fetch.eqb lhs rhs eqb.
+
+Lemma feqb_reflection (lhs rhs: @Fetch Byte):
+  feqb lhs rhs = true -> lhs = rhs.
+Proof.
+  intros. unfold feqb in H. unfold eqb in H.
+  destruct lhs.
+    destruct rhs; [| discriminate H | discriminate H]. 
+      apply eqb_reflection in H. rewrite H. reflexivity.
+    destruct rhs; [discriminate H | | discriminate H].
+      apply N.eqb_eq in H. rewrite H. reflexivity.
+    discriminate H.
+Qed.
