ByteData.v
@@ -2,44 +2,44 @@ Require Import Coq.ZArith.ZArith.
 Require Import FSets.FMaps.
 Require Import FSets.FMapAVL.
 
+Require Import Byte.
 Require Import Fetch.
 
-Open Local Scope Z.
+Open Local Scope N.
 
 (* instantiation of the AVL module that implements the finite map interface *)
-Module MZ := FSets.FMapAVL.Make Z_as_OT.
+Module MN := FSets.FMapAVL.Make N_as_OT.
 
 (* the type of finite maps from Z to Z *)
-Definition Map_Z_Z : Type := MZ.t Z.
+Definition Map_N_Byte : Type := MN.t Byte.
 
 (* lookup in a finite map *)
-Definition find k (m: Map_Z_Z) := MZ.find k m.
+Definition find k (m: Map_N_Byte) := MN.find k m.
 
 (* create a new finite map by adding/overwriting an element with an existing
    finite map *)
-Definition update (p: Z*Z) (m: Map_Z_Z) := MZ.add (fst p) (snd p) m.
+Definition update (p: N*Byte) (m: Map_N_Byte) := MN.add (fst p) (snd p) m.
 
 (* notation for building finite maps *)
 (* k |-> v   says that key k maps to value v *)
 Notation "k |-> v" := (pair k v) (at level 60).
-Notation "[ ]" := (MZ.empty Z).
+Notation "[ ]" := (MN.empty Byte).
 Notation "[ p1 , .. , pn ]" := (update p1 .. (update pn []) .. ).
 
-Definition ByteString := list Z.
-Definition ByteData := Z -> (@Fetch Z).
+Definition ByteData := N -> (@Fetch Byte).
 Definition Disk := ByteData.
 
 Bind Scope ByteData_scope with Disk.
 
-Definition Disk_of_Map_Z_Z (map: Map_Z_Z) : Disk :=
-  fun (key: Z) => match (find key map) with
+Definition Disk_of_Map_N_Byte (map: Map_N_Byte) : Disk :=
+  fun (key: N) => match (find key map) with
   | error => MissingAt key
   | value v => Found v
   end.
 
-Coercion Disk_of_Map_Z_Z : Map_Z_Z >-> Disk.
+Coercion Disk_of_Map_N_Byte : Map_N_Byte >-> Disk.
 
 (* Change the "zero" index; i.e. "shift" the bytes *)
-Definition shift (bytes: ByteData) (shiftAmount index: Z) 
+Definition shift (bytes: ByteData) (shiftAmount index: N) 
   : Fetch :=
   bytes (shiftAmount + index).
