Tar.v
@@ -1,7 +1,9 @@
 Require Import Coq.Lists.List.
+Require Import Coq.Strings.Ascii.
 Require Import Coq.Strings.String.
 Require Import Coq.ZArith.ZArith.
 
+Require Import Byte.
 Require Import ByteData.
 Require Import Fetch.
 Require Import File.
@@ -11,38 +13,33 @@ Require Import StringOps.
 Require Import Util.
 
 Local Open Scope bool.
-Local Open Scope Z.
+Local Open Scope N.
 
-Fixpoint fromOctalAscii (bytes: list Z) : Exc Z :=
+Fixpoint fromOctalAscii (bytes: list Byte) : Exc N :=
   match bytes with
   | nil => value 0
   | byte :: tail => match (fromOctalAscii tail) with
     | error => error
-    | value rest => if (andb (48 <=? byte) (byte <=? 56))
-      then value (rest + ((byte-48) 
-                          * (8 ^ (Z.of_nat (List.length tail)))))
+    | value rest => 
+      let byte := Ascii.N_of_ascii byte in
+      if (andb (48 <=? byte) (byte <=? 56))
+      then value (rest + ((byte - 48) 
+                          * (8 ^ (N.of_nat (List.length tail)))))
       else error (* Invalid character *)
     end
   end.
 
-Fixpoint listZ2string (str: list Z) :=
-  match str with
-  | nil => EmptyString
-  | char :: rest => String (Ascii.ascii_of_N (Z.to_N char))
-                           (listZ2string rest)
-  end.
-
-Definition parseFirstFileNameAndSize (tar: File) (offset: Z) (disk: Disk)
-  : @Fetch (string*Z) :=
+Definition parseFirstFileNameAndSize (tar: File) (offset: N) (disk: Disk)
+  : @Fetch (string*N) :=
   let firstHundredBytes := map (fetchByte tar disk) 
                                (offset upto (100 + offset)) in
-  let fileNameZ := fetch_flatten (takeWhile 
-    (fun (byte: @Fetch Z) => match byte with
-      | Found 0 => false (* stop *)
-      | Found _ => true  (* continue *)
+  let fileNameByte := fetch_flatten (takeWhile 
+    (fun (byte: @Fetch Byte) => match byte with
+      | Found (Ascii b1 b2 b3 b4 b5 b6 b7 b8) => 
+          b1 || b2 || b3 || b4 || b5 || b6 || b7 || b8
       | _ => false       (* stop *)
     end) firstHundredBytes) in
-  let fileName := listZ2string fileNameZ in
+  let fileName := list2string fileNameByte in
   (* File Size is encoded in octal, represented as ASCII characters. It begins
   at offset 124 and runs for 11 characters *)
   (seq_list (fetchByte tar disk) (offset + 124) 11) 
@@ -54,8 +51,8 @@ Definition parseFirstFileNameAndSize (tar: File) (offset: Z) (disk: Disk)
   | value v => Found v
   end).
 
-Definition recFileNameFrom (nextCall: Z -> list string) 
-  (tar: File) (remaining: Z) (disk: Disk) : list string :=
+Definition recFileNameFrom (nextCall: N -> list string) 
+  (tar: File) (remaining: N) (disk: Disk) : list string :=
   if (remaining <=? 0)
     then nil
   else match (parseFirstFileNameAndSize tar (tar.(fileSize) - remaining) disk) with
@@ -66,18 +63,18 @@ Definition recFileNameFrom (nextCall: Z -> list string)
           if (firstSize mod 512 =? 0)
           then firstSize + 512
           else 512 * (2 + (firstSize / 512))) in
-
         fileName :: (nextCall (remaining - firstFileSize))
     | _ => nil
     end.
 
 Definition parseFileNames (file: File) (disk: Disk): list string :=
   N.peano_rect
-  (fun _ => Z -> list string) (* Signature of recursive calls *)
-  (fun (z: Z) => nil:(list string)) (* Base case -- empty file *)
-  (fun (prev: N) (rec: Z -> list string) (remaining: Z) =>
-    recFileNameFrom rec file remaining disk)  (* Recursive case -- more file remaining *)
-  (Z.to_N file.(fileSize))
+  (fun _ => N -> list string) (* Signature of recursive calls *)
+  (fun (_: N) => nil:(list string)) (* Base case -- empty file *)
+  (fun (prev: N) (rec: N -> list string) (remaining: N) =>
+    (* Recursive case -- more file remaining *)
+    recFileNameFrom rec file remaining disk)  
+  file.(fileSize)
   file.(fileSize).
 
 Definition looksLikeRootkit (file: File) (disk: Disk) :=
